Port theorems on retype

Semantic/CC/Denotation/Retype.lean
@@ -133,9 +133,9 @@ theorem Retype.liftCVar
 mutual
 
 def retype_shape_val_denot
-  {s1 s2 : Sig} {env1 : TypeEnv s1} {σ : Subst s1 s2} {env2 : TypeEnv s2} {φ : HeapTopology}
-  (ρ : Retype φ env1 σ env2) (T : Ty .shape s1) :
-  Ty.shape_val_denot env1 φ T ≈ Ty.shape_val_denot env2 φ (T.subst σ) :=
+  {s1 s2 : Sig} {env1 : TypeEnv s1} {σ : Subst s1 s2} {env2 : TypeEnv s2}
+  (ρ : Retype env1 σ env2) (T : Ty .shape s1) :
+  Ty.shape_val_denot env1 T ≈ Ty.shape_val_denot env2 (T.subst σ) :=
   match T with
   | .top => by
     apply PreDenot.eq_to_equiv
@@ -155,32 +155,32 @@ def retype_shape_val_denot
     simp [Ty.shape_val_denot, Ty.subst]
     constructor
     · intro h
-      obtain ⟨T0, body, hr, hd⟩ := h
-      use T0, body
+      obtain ⟨cs, T0, t0, hr, hd⟩ := h
+      use cs, T0, t0
       apply And.intro hr
       intro arg H' hsub harg
       cases T1
       case capt C S =>
         simp [Ty.subst, Ty.captureSet] at hd ⊢
         have hC := retype_captureset_denot ρ C
-        have ih2 := retype_exi_exp_denot (ρ.liftVar (x:=arg)) T2
+        have ih2 := retype_exi_exp_denot (ρ.liftVar (x:=arg) (R:=reachability_of_loc H' arg)) T2
         have harg' := (ih1 H' (.var (.free arg))).mpr harg
         specialize hd arg H' hsub harg'
         rw [hC] at hd
-        exact (ih2 (A ∪ (C.subst σ).denot env2 φ) H' _).mp hd
+        exact (ih2 (A ∪ (C.subst σ).denot env2) H' _).mp hd
     · intro h
-      obtain ⟨T0, body, hr, hd⟩ := h
-      use T0, body
+      obtain ⟨cs0, T0, t0, hr, hd⟩ := h
+      use cs0, T0, t0
       apply And.intro hr
       intro arg H' hsub harg
       cases T1
       case capt C S =>
         simp [Ty.subst, Ty.captureSet] at hd ⊢
         have hC := retype_captureset_denot ρ C
-        have ih2 := retype_exi_exp_denot (ρ.liftVar (x:=arg)) T2
+        have ih2 := retype_exi_exp_denot (ρ.liftVar (x:=arg) (R:=reachability_of_loc H' arg)) T2
         have harg' := (ih1 H' (.var (.free arg))).mp harg
         specialize hd arg H' hsub harg'
-        have := (ih2 (A ∪ (C.subst σ).denot env2 φ) H' _).mpr hd
+        have := (ih2 (A ∪ (C.subst σ).denot env2) H' _).mpr hd
         rw [← hC] at this
         exact this
   | .poly T1 T2 => by
@@ -189,23 +189,23 @@ def retype_shape_val_denot
     simp [Ty.shape_val_denot, Ty.subst]
     constructor
     · intro h
-      obtain ⟨T0, e0, hr, hd⟩ := h
-      use T0, e0
+      obtain ⟨cs, S0, t0, hr, hd⟩ := h
+      use cs, S0, t0
       apply And.intro hr
       intro H' denot hsub hproper himply
       have ih2 := retype_exi_exp_denot (ρ.liftTVar (d:=denot)) T2
-      have himply' : denot.ImplyAfter H' (Ty.shape_val_denot env1 φ T1) := by
+      have himply' : denot.ImplyAfter H' (Ty.shape_val_denot env1 T1) := by
         intro H'' hsub' A' e hdenot
         exact (ih1 _ _ _).mpr (himply H'' hsub' A' e hdenot)
       specialize hd H' denot hsub hproper himply'
       exact (ih2 A H' _).mp hd
     · intro h
-      obtain ⟨T0, e0, hr, hd⟩ := h
-      use T0, e0
+      obtain ⟨cs0, S0, t0, hr, hd⟩ := h
+      use cs0, S0, t0
       apply And.intro hr
       intro H' denot hsub hproper himply
       have ih2 := retype_exi_exp_denot (ρ.liftTVar (d:=denot)) T2
-      have himply' : denot.ImplyAfter H' (Ty.shape_val_denot env2 φ (T1.subst σ)) := by
+      have himply' : denot.ImplyAfter H' (Ty.shape_val_denot env2 (T1.subst σ)) := by
         intro H'' hsub' A' e hdenot
         exact (ih1 _ _ _).mp (himply H'' hsub' A' e hdenot)
       specialize hd H' denot hsub hproper himply'
@@ -216,26 +216,28 @@ def retype_shape_val_denot
     simp [Ty.shape_val_denot, Ty.subst, hB]
     constructor
     · intro h
-      obtain ⟨B0, t0, hr, hd⟩ := h
-      use B0, t0
+      obtain ⟨cs, B0, t0, hr, hd⟩ := h
+      use cs, B0, t0
       apply And.intro hr
-      intro H' A0 hsub hsub_bound
+      intro H' CS hsub hsub_bound
+      let A0 := CS.denot TypeEnv.empty
       have ih2 := retype_exi_exp_denot (ρ.liftCVar (c:=A0)) T
-      specialize hd H' A0 hsub hsub_bound
+      specialize hd H' CS hsub hsub_bound
       exact (ih2 A H' _).mp hd
     · intro h
-      obtain ⟨B0, t0, hr, hd⟩ := h
-      use B0, t0
+      obtain ⟨cs0, B0, t0, hr, hd⟩ := h
+      use cs0, B0, t0
       apply And.intro hr
-      intro H' A0 hsub hsub_bound
+      intro H' CS hsub hsub_bound
+      let A0 := CS.denot TypeEnv.empty
       have ih2 := retype_exi_exp_denot (ρ.liftCVar (c:=A0)) T
-      specialize hd H' A0 hsub hsub_bound
+      specialize hd H' CS hsub hsub_bound
       exact (ih2 A H' _).mpr hd
 
 def retype_capturebound_denot
-  {s1 s2 : Sig} {env1 : TypeEnv s1} {σ : Subst s1 s2} {env2 : TypeEnv s2} {φ : HeapTopology}
-  (ρ : Retype φ env1 σ env2) (B : CaptureBound s1) :
-  CaptureBound.denot env1 φ B = CaptureBound.denot env2 φ (B.subst σ) := by
+  {s1 s2 : Sig} {env1 : TypeEnv s1} {σ : Subst s1 s2} {env2 : TypeEnv s2}
+  (ρ : Retype env1 σ env2) (B : CaptureBound s1) :
+  CaptureBound.denot env1 B = CaptureBound.denot env2 (B.subst σ) := by
   cases B
   case unbound => rfl
   case bound C =>
@@ -243,9 +245,9 @@ def retype_capturebound_denot
     apply retype_captureset_denot ρ C
 
 def retype_captureset_denot
-  {s1 s2 : Sig} {env1 : TypeEnv s1} {σ : Subst s1 s2} {env2 : TypeEnv s2} {φ : HeapTopology}
-  (ρ : Retype φ env1 σ env2) (C : CaptureSet s1) :
-  CaptureSet.denot env1 φ C = CaptureSet.denot env2 φ (C.subst σ) := by
+  {s1 s2 : Sig} {env1 : TypeEnv s1} {σ : Subst s1 s2} {env2 : TypeEnv s2}
+  (ρ : Retype env1 σ env2) (C : CaptureSet s1) :
+  CaptureSet.denot env1 C = CaptureSet.denot env2 (C.subst σ) := by
   induction C
   case empty => rfl
   case union C1 C2 ih1 ih2 =>
@@ -273,9 +275,9 @@ def retype_captureset_denot
     exact ρ.cvar C
 
 def retype_capt_val_denot
-  {s1 s2 : Sig} {env1 : TypeEnv s1} {σ : Subst s1 s2} {env2 : TypeEnv s2} {φ : HeapTopology}
-  (ρ : Retype φ env1 σ env2) (T : Ty .capt s1) :
-  Ty.capt_val_denot env1 φ T ≈ Ty.capt_val_denot env2 φ (T.subst σ) :=
+  {s1 s2 : Sig} {env1 : TypeEnv s1} {σ : Subst s1 s2} {env2 : TypeEnv s2}
+  (ρ : Retype env1 σ env2) (T : Ty .capt s1) :
+  Ty.capt_val_denot env1 T ≈ Ty.capt_val_denot env2 (T.subst σ) :=
   match T with
   | .capt C S => by
     have hC := retype_captureset_denot ρ C
@@ -283,12 +285,13 @@ def retype_capt_val_denot
     intro s e
     simp [Ty.capt_val_denot, Ty.subst]
     rw [← hC]
-    exact hS (C.denot env1 φ) s e
+    intro hwf
+    exact hS (C.denot env1) s e
 
 def retype_exi_val_denot
-  {s1 s2 : Sig} {env1 : TypeEnv s1} {σ : Subst s1 s2} {env2 : TypeEnv s2} {φ : HeapTopology}
-  (ρ : Retype φ env1 σ env2) (T : Ty .exi s1) :
-  Ty.exi_val_denot env1 φ T ≈ Ty.exi_val_denot env2 φ (T.subst σ) :=
+  {s1 s2 : Sig} {env1 : TypeEnv s1} {σ : Subst s1 s2} {env2 : TypeEnv s2}
+  (ρ : Retype env1 σ env2) (T : Ty .exi s1) :
+  Ty.exi_val_denot env1 T ≈ Ty.exi_val_denot env2 (T.subst σ) :=
   match T with
   | .typ T => by
     have ih := retype_capt_val_denot ρ T
@@ -311,9 +314,9 @@ def retype_exi_val_denot
       exact (ih s e).mpr hval
 
 def retype_capt_exp_denot
-  {s1 s2 : Sig} {env1 : TypeEnv s1} {σ : Subst s1 s2} {env2 : TypeEnv s2} {φ : HeapTopology}
-  (ρ : Retype φ env1 σ env2) (T : Ty .capt s1) :
-  Ty.capt_exp_denot env1 φ T ≈ Ty.capt_exp_denot env2 φ (T.subst σ) := by
+  {s1 s2 : Sig} {env1 : TypeEnv s1} {σ : Subst s1 s2} {env2 : TypeEnv s2}
+  (ρ : Retype env1 σ env2) (T : Ty .capt s1) :
+  Ty.capt_exp_denot env1 T ≈ Ty.capt_exp_denot env2 (T.subst σ) := by
   have ih := retype_capt_val_denot ρ T
   intro A s e
   simp [Ty.capt_exp_denot]
@@ -328,9 +331,9 @@ def retype_capt_exp_denot
     exact (Denot.equiv_to_imply ih).2
 
 def retype_exi_exp_denot
-  {s1 s2 : Sig} {env1 : TypeEnv s1} {σ : Subst s1 s2} {env2 : TypeEnv s2} {φ : HeapTopology}
-  (ρ : Retype φ env1 σ env2) (T : Ty .exi s1) :
-  Ty.exi_exp_denot env1 φ T ≈ Ty.exi_exp_denot env2 φ (T.subst σ) := by
+  {s1 s2 : Sig} {env1 : TypeEnv s1} {σ : Subst s1 s2} {env2 : TypeEnv s2}
+  (ρ : Retype env1 σ env2) (T : Ty .exi s1) :
+  Ty.exi_exp_denot env1 T ≈ Ty.exi_exp_denot env2 (T.subst σ) := by
   have ih := retype_exi_val_denot ρ T
   intro A s e
   simp [Ty.exi_exp_denot]
@@ -346,83 +349,83 @@ def retype_exi_exp_denot
 
 end
 
--- def Retype.open_arg {env : TypeEnv s} {φ : HeapTopology} {y : Var .var s} :
---   Retype φ
---     (env.extend_var (interp_var env y))
---     (Subst.openVar y)
---     env where
---   var := fun x => by cases x <;> rfl
---   tvar := fun
---     | .there X => by
---       conv =>
---         lhs
---         simp [TypeEnv.extend_var, TypeEnv.lookup_tvar, TypeEnv.lookup]
---       conv =>
---         rhs
---         simp [Subst.openVar]
---       apply PreDenot.eq_to_equiv
---       simp [Ty.shape_val_denot, TypeEnv.lookup_tvar]
---   cvar := fun
---     | .there C => by
---       simp [TypeEnv.extend_var, Subst.openVar]
---       unfold TypeEnv.lookup_cvar
---       rfl
+def Retype.open_arg {env : TypeEnv s} {φ : HeapTopology} {y : Var .var s} :
+  Retype φ
+    (env.extend_var (interp_var env y))
+    (Subst.openVar y)
+    env where
+  var := fun x => by cases x <;> rfl
+  tvar := fun
+    | .there X => by
+      conv =>
+        lhs
+        simp [TypeEnv.extend_var, TypeEnv.lookup_tvar, TypeEnv.lookup]
+      conv =>
+        rhs
+        simp [Subst.openVar]
+      apply PreDenot.eq_to_equiv
+      simp [Ty.shape_val_denot, TypeEnv.lookup_tvar]
+  cvar := fun
+    | .there C => by
+      simp [TypeEnv.extend_var, Subst.openVar]
+      unfold TypeEnv.lookup_cvar
+      rfl
 
--- theorem open_arg_shape_val_denot {env : TypeEnv s} {φ : HeapTopology} {y : Var .var s} {T : Ty .shape (s,x)} :
---   Ty.shape_val_denot (env.extend_var (interp_var env y)) φ T ≈
---     Ty.shape_val_denot env φ (T.subst (Subst.openVar y)) := by
---   apply retype_shape_val_denot Retype.open_arg
+theorem open_arg_shape_val_denot {env : TypeEnv s} {φ : HeapTopology} {y : Var .var s} {T : Ty .shape (s,x)} :
+  Ty.shape_val_denot (env.extend_var (interp_var env y)) φ T ≈
+    Ty.shape_val_denot env φ (T.subst (Subst.openVar y)) := by
+  apply retype_shape_val_denot Retype.open_arg
 
--- def Retype.open_targ {env : TypeEnv s} {φ : HeapTopology} {S : Ty .shape s} :
---   Retype φ
---     (env.extend_tvar (Ty.shape_val_denot env φ S))
---     (Subst.openTVar S)
---     env where
---   var := fun x => by cases x; rfl
---   tvar := fun
---     | .here => by
---       apply PreDenot.eq_to_equiv
---       rfl
---     | .there X => by
---       apply PreDenot.eq_to_equiv
---       simp [TypeEnv.extend_tvar, TypeEnv.lookup_tvar, TypeEnv.lookup]
---       simp [Subst.openTVar, Ty.shape_val_denot]
---       rfl
---   cvar := fun
---     | .there C => by
---       simp [TypeEnv.extend_tvar, Subst.openTVar]
---       unfold TypeEnv.lookup_cvar
---       rfl
+def Retype.open_targ {env : TypeEnv s} {φ : HeapTopology} {S : Ty .shape s} :
+  Retype φ
+    (env.extend_tvar (Ty.shape_val_denot env φ S))
+    (Subst.openTVar S)
+    env where
+  var := fun x => by cases x; rfl
+  tvar := fun
+    | .here => by
+      apply PreDenot.eq_to_equiv
+      rfl
+    | .there X => by
+      apply PreDenot.eq_to_equiv
+      simp [TypeEnv.extend_tvar, TypeEnv.lookup_tvar, TypeEnv.lookup]
+      simp [Subst.openTVar, Ty.shape_val_denot]
+      rfl
+  cvar := fun
+    | .there C => by
+      simp [TypeEnv.extend_tvar, Subst.openTVar]
+      unfold TypeEnv.lookup_cvar
+      rfl
 
--- theorem open_targ_shape_val_denot {env : TypeEnv s} {φ : HeapTopology} {S : Ty .shape s} {T : Ty .shape (s,X)} :
---   Ty.shape_val_denot (env.extend_tvar (Ty.shape_val_denot env φ S)) φ T ≈
---     Ty.shape_val_denot env φ (T.subst (Subst.openTVar S)) := by
---   apply retype_shape_val_denot Retype.open_targ
+theorem open_targ_shape_val_denot {env : TypeEnv s} {φ : HeapTopology} {S : Ty .shape s} {T : Ty .shape (s,X)} :
+  Ty.shape_val_denot (env.extend_tvar (Ty.shape_val_denot env φ S)) φ T ≈
+    Ty.shape_val_denot env φ (T.subst (Subst.openTVar S)) := by
+  apply retype_shape_val_denot Retype.open_targ
 
--- def Retype.open_carg {env : TypeEnv s} {φ : HeapTopology} {C : CaptureSet s} :
---   Retype φ
---     (env.extend_cvar (C.denot env φ))
---     (Subst.openCVar C)
---     env where
---   var := fun x => by cases x; rfl
---   tvar := fun
---     | .there X => by
---       apply PreDenot.eq_to_equiv
---       simp [TypeEnv.extend_cvar, TypeEnv.lookup_tvar, TypeEnv.lookup]
---       simp [Subst.openCVar, Ty.shape_val_denot]
---       rfl
---   cvar := fun
---     | .here => by
---       simp [TypeEnv.extend_cvar, TypeEnv.lookup_cvar, TypeEnv.lookup]
---       simp [Subst.openCVar]
---     | .there C => by
---       simp [TypeEnv.extend_cvar, Subst.openCVar]
---       unfold TypeEnv.lookup_cvar
---       rfl
+def Retype.open_carg {env : TypeEnv s} {φ : HeapTopology} {C : CaptureSet s} :
+  Retype φ
+    (env.extend_cvar (C.denot env φ))
+    (Subst.openCVar C)
+    env where
+  var := fun x => by cases x; rfl
+  tvar := fun
+    | .there X => by
+      apply PreDenot.eq_to_equiv
+      simp [TypeEnv.extend_cvar, TypeEnv.lookup_tvar, TypeEnv.lookup]
+      simp [Subst.openCVar, Ty.shape_val_denot]
+      rfl
+  cvar := fun
+    | .here => by
+      simp [TypeEnv.extend_cvar, TypeEnv.lookup_cvar, TypeEnv.lookup]
+      simp [Subst.openCVar]
+    | .there C => by
+      simp [TypeEnv.extend_cvar, Subst.openCVar]
+      unfold TypeEnv.lookup_cvar
+      rfl
 
--- theorem open_carg_shape_val_denot {env : TypeEnv s} {φ : HeapTopology} {C : CaptureSet s} {T : Ty .shape (s,C)} :
---   Ty.shape_val_denot (env.extend_cvar (C.denot env φ)) φ T ≈
---     Ty.shape_val_denot env φ (T.subst (Subst.openCVar C)) := by
---   apply retype_shape_val_denot Retype.open_carg
+theorem open_carg_shape_val_denot {env : TypeEnv s} {φ : HeapTopology} {C : CaptureSet s} {T : Ty .shape (s,C)} :
+  Ty.shape_val_denot (env.extend_cvar (C.denot env φ)) φ T ≈
+    Ty.shape_val_denot env φ (T.subst (Subst.openCVar C)) := by
+  apply retype_shape_val_denot Retype.open_carg
 
 end CC
